feat(library/init/meta): support mutual coinductive predicates

library/init/meta/coinductive_predicates.lean
@@ -4,13 +4,10 @@ Released under Apache 2.0 license as described in the file LICENSE.
 Author: Johannes Hölzl (CMU)
 -/
 prelude
-import init.meta.expr init.meta.tactic
+import init.meta.expr init.meta.tactic init.meta.constructor_tactic
 
 namespace expr
 open expr
-
-meta def replace_with (e : expr) (s : expr) (s' : expr) : expr :=
-e.replace $ λc d, if c = s then some s' else none
 
 meta def local_binder_info : expr → binder_info
 | (local_const x n bi t) := bi
@@ -58,135 +55,223 @@ The coinductive predicate `pred`:
 where
   `u` is a list of universe parameters
   `A` is a list of global parameters
-  `a` are the indices
-  `r` is a list of introduction rules
-  `b` is a list of parameters for each rule in `r`
+  `pred` is a list predicates to be defined
+  `a` are the indices for each `pred`
+  `r` is a list of introduction rules for each `pred`
+  `b` is a list of parameters for each rule in `r` and `pred`
   `p` is are the instances of `a` using `A` and `b`
 
 `pred` is compiled to the following defintions:
 
-  inductive {u} pred.functional (A) (f : a → Prop) : a → Prop
-  | r : ∀a f, b[pred/f] → pred.functional a f p
+  inductive {u} pred.functional (A) ([pred'] : a → Prop) : a → Prop
+  | r : ∀a [f], b[pred/pred'] → pred.functional a [f] p
 
-  lemma {u} pred.functional.mono (A) (f f' : a → Prop) (h : ∀b, f b → f' b) :
-    ∀p, pred.functional A f p → pred.functional A f' p :=
+  lemma {u} pred.functional.mono (A) ([pred₁] [pred₂] : a → Prop) [(h : ∀b, pred₁ b → pred₂ b)] :
+    ∀p, pred.functional A pred₁ p → pred.functional A pred₂ p :=
   pred.functional.rec A f (pred.functional A f')
     (take p, pred.functional.r A f' p[mono with h])
 
-  def {u} pred (A) (a) : Prop :=
-  ∃f, (∀a, f a → pred.functional A f a) ∧ f a
+  def {u} pred_i (A) (a) : Prop :=
+  ∃[pred'], (Λi, ∀a, pred_i a → pred_i.functional A [pred] a) ∧ pred'_i a
 
-  lemma {u} pred.corec_functional (A) (C : a → Prop) (h : ∀a, C a → pred.functional A C a) :
-    ∀a, C a → pred A a :=
-  take a ha, ⟨C, h, ha⟩
+  lemma {u} pred_i.corec_functional (A) [(C : a → Prop)] (h : ∀[a], [C a] → pred.functional A [C] a) :
+    ∀a, C_i a → pred_i A a :=
+  take a ha, ⟨[C], [h], ha⟩
 
-  lemma {u} pred.destruct (A) (a) : pred A a → pred.functional A (pred A) a :=
+  lemma {u} pred_i.destruct (A) (a) : pred A a → pred.functional A [pred A] a :=
   Exists.rec (a → Prop) (λf, (∀a, f a → pred.functional A f a) ∧ f a)
     (pred.functional A (pred A a) a) h $
   take f, and.rec.{0} (∀a, f a → pred.functional A f a) (f a) $
     assume h₁ : ∀a, f a → pred.functional A f a, assume h₂ : f a,
     pred.functional.mono A f (pred A) (pred.corec_functional A f h₁) a (h₁ a h₂))
 
-  lemma {u} pred.construct (A) : ∀a, pred.functional A (pred A) a → pred A a :=
+  lemma {u} pred_i.construct (A) : ∀a, pred_i.functional A [pred A] a → pred_i A a :=
   pred.corec_functional A (pred.functional A (pred A))
     (pred.functional.mono A (pred A) (pred.functional A (pred A)) (pred.destruct A))
 
-  lemma {u} pred.r (A) (b) : pred A p :=
-  pred.construct A p $ pred.functional.r A (pred A) b
-
+  lemma {u} pred.r (A) (b) : pred_i A p :=
+  pred_i.construct A p $ pred_i.functional.r A [pred A] b
 -/
 
+open level expr tactic
+
+namespace add_coinductive_predicate
+
+/- private -/ meta structure pred_predata : Type :=
+(u_params : list level)
+(params   : list expr)
+(pd_name  : name)
+(pred     : expr)
+(type     : expr)
+(intros   : list (name × expr))
+(locals   : list expr)
+(f₁ f₂    : expr)
+(u_f      : level)
+(func     : expr)
+
+namespace pred_predata
+
+meta def f₁_l (pd : pred_predata) : expr :=
+pd.f₁.app_of_list pd.locals
+
+meta def f₂_l (pd : pred_predata) : expr :=
+pd.f₂.app_of_list pd.locals
+
+meta def func_g (pd : pred_predata) : expr :=
+pd.func.app_of_list $ pd.params
+
+meta def pred_g (pd : pred_predata) : expr :=
+pd.pred.app_of_list $ pd.params
+
+meta def le (pd : pred_predata) (f₁ f₂ : expr) : expr :=
+(imp (f₁.app_of_list pd.locals) (f₂.app_of_list pd.locals)).pis pd.locals
+
+meta def corec (pd : pred_predata) : expr :=
+const (pd.pd_name ++ "corec_functional") pd.u_params
+
+meta def mono (pd : pred_predata) : expr :=
+const (pd.func.const_name ++ "mono") pd.u_params
+
+meta def construct (pd : pred_predata) : expr :=
+const (pd.pd_name ++ "construct") pd.u_params
+
+meta def destruct (pd : pred_predata) : expr :=
+const (pd.pd_name ++ "destruct") pd.u_params
+
+end pred_predata
+
+end add_coinductive_predicate
+
+open add_coinductive_predicate
+
 meta def add_coinductive_predicate
-  (n : name) (us : list name) (p : nat) (type : expr) (irules : list (name × expr)) : command := do
-  let us' := us.map param,
+  (u_params : list name) (params : list expr) (preds : list $ expr × list expr) : command := do
+  let params_names := params.map local_pp_name,
+  let u_params' := u_params.map param,
 
-  /- introduce locals to represent global parameters -/
-  (gs, type') ← mk_local_pisn type p,
-  (ls, `(Prop)) ← mk_local_pis type',
-  let gs_names := gs.map local_pp_name,
-  let ls_names := ls.map local_pp_name,
+  pds ← preds.mmap (λ⟨c, is⟩, do
+    (ls, `(Prop)) ← mk_local_pis c.local_type,
+    f₁ ← mk_local_def `f₁ c.local_type,
+    f₂ ← mk_local_def `f₂ c.local_type,
+    sort u_f ← infer_type f₁ >>= infer_type,
+    let func : expr := const (c.local_pp_name ++ "functional") u_params',
+    return {tactic.add_coinductive_predicate.pred_predata .
+      pd_name := c.local_pp_name,
+      pred := const c.local_pp_name u_params', type := c.local_type,
+      intros := is.map (λi, (i.local_pp_name, i.local_type)),
+      locals := ls, params := params, u_params := u_params',
+      f₁ := f₁, f₂ := f₂, u_f := u_f, func := func}),
 
-  -- vv this will be two lists of functions to support mutual induction
-  f ← mk_local_def `f type',
-  f₂ ← mk_local_def `f' type',
-  sort u_f ← infer_type f >>= infer_type,
+  let f₁ := pds.map pred_predata.f₁,
+  let f₂ := pds.map pred_predata.f₂,
 
-  /- define often occuring subterms -/
-  let pred : expr := const n us',
-  let pred_g      := pred.app_of_list gs,
-  let pred_gl     := pred_g.app_of_list ls,
+  /- Introduce all functionals -/
+  pds.mmap (λpd:pred_predata, do
+    let func_f₁ := pd.func_g.app_of_list $ f₁,
+    let func_f₂ := pd.func_g.app_of_list $ f₂,
 
-  let func_type   := type'.pis $ gs ++ [f],
-  let func_name   := n ++ "functional",
-  let func : expr := const func_name us',
-  let func_g      := func.app_of_list gs,
-  let func_f      := func_g f,
-  let func_f₂     := func_g f₂,
-  let func_pred_l := func.app_of_list $ gs ++ [pred_g] ++ ls,
+    /- Define functional for `pd` as inductive predicate -/
+    func_intros ← pd.intros.mmap (λ⟨nr, t⟩, do
+      (bs, t') ← mk_local_pis t,
+      (name.mk_string sub p) ← return $ nr,
+      let bs := bs.map $ expr.instantiate_locals $ pds.map (λpd:pred_predata, (pd.pd_name, pd.f₁)),
+      let t' := expr.instantiate_local pd.pd_name (pd.func.app_of_list $ params ++ f₁) t',
+      return ((p ++ "functional") ++ sub, t'.pis $ params ++ f₁ ++ bs)),
+    let func_type := pd.type.pis $ params ++ f₁,
+    add_inductive pd.func.const_name u_params (params.length + preds.length) func_type func_intros,
 
-  let f_l         := f.app_of_list ls,
-  let f₂_l        := f₂.app_of_list ls,
-  let f_le_func := (f_l.imp $ func_f.app_of_list ls).pis ls,
-
-  /- define `functional` as inductive predicate -/
-  func_intros   ← irules.mmap (λ⟨nr, t⟩, do
-    (ls, t') ← drop_pis gs t >>= mk_local_pis,
-    let ls' := ls.map $ λe, e.replace_with pred_g f,
-    let t'  := t'.replace_with pred_g func_f,
-    (name.mk_string sub p) ← return $ nr,
-    return ((p ++ "functional") ++ sub, t'.pis $ gs ++ [f] ++ ls')),
-  add_inductive func_name us (p + 1) func_type func_intros,
-
-  /- prove monotonicity of `functional` -/
-  let mono_func : expr := (imp (func_f.app_of_list ls) (func_f₂.app_of_list ls)).pis ls,
-  mono ← add_theorem_by (func_name ++ "mono") us
-    ((imp ((imp f_l f₂_l).pis ls) mono_func).pis $ gs ++ [f, f₂]) (do
-      gs ← intro_lst gs_names,
-      [f₁, f₂, hf] ← intro_lst [`f₁, `f₂, `hf],
-      m ← mk_const (func_name ++ "rec"), -- `rec`'s universes are not always `us`, e.g. eq, wf, false
-      apply $ m.app_of_list gs, -- somhow `induction` / `cases` doesn't work?
+    /- Prove monotonicity rule -/
+    let mono_type :=
+      pds.foldl (λc (pd:pred_predata), ((pd.le pd.f₁ pd.f₂).imp c).pis [pd.f₁, pd.f₂]) $
+      pd.le func_f₁ func_f₂,
+    add_theorem_by (pd.func.const_name ++ "mono") u_params (mono_type.pis $ params) (do
+      params ← intro_lst params_names,
+      hf ← pds.mmap (λpd, do
+        [f₁, f₂, hf] ← intro_lst [`f₁, `f₂, `hf],
+        return (f₂, hf)),
+      let fs₂ := hf.map prod.fst,
+      let hfs := hf.map prod.snd,
+      m ← mk_const (pd.func.const_name ++ "rec"),
+        -- ^^ `rec`'s universes are not always `u_params`, e.g. eq, wf, false
+      apply $ m.app_of_list params, -- somhow `induction` / `cases` doesn't work?
       focus $ func_intros.map (λ⟨n, t⟩, do
         bs ← intros,
-        ms ← apply_core ((const n us').app_of_list $ gs ++ [f₂]) { all := tt },
-        gs ← (ms.zip bs).mfilter (λ⟨m, d⟩, is_assigned m),
-        focus $ gs.map (λ⟨m, d⟩, apply d <|> (apply hf >> apply d)))),
+        ms ← apply_core ((const n u_params').app_of_list $ params ++ fs₂) { all := tt },
+        params ← (ms.zip bs).mfilter (λ⟨m, d⟩, is_assigned m),
+        focus $ params.map (λ⟨m, d⟩, apply d <|> first (hfs.map $ λ hf, apply hf >> apply d))))),
 
-  /- define `pred` as fixed point of `functional` -/
-  add_decl $ mk_definition n us type $
-    (((const `Exists [u_f] : expr) type' ((`(and) f_le_func f_l).lambdas [f])).lambdas $ gs ++ ls),
+  pds.mmap (λpd:pred_predata, do
+    let func_f := pd.func_g.app_of_list $ pds.map pred_predata.f₁,
 
-  /- prove `corec_functional` rule -/
-  corec ← add_theorem_by (n ++ "corec_functional") us
-    ((f_le_func.imp ((imp f_l pred_gl).pis ls)).pis $ gs ++ [f]) (do
-      intro_lst gs_names, [C, hC] ← intro_lst [`C, `hC], intro_lst ls_names, hls ← intro `hls,
-      refine ``(exists.intro %%C (and.intro %%hC %%hls))),
+    /- define final predicate -/
+    pred_body ← (do
+      corec ← pds.mfoldl
+        (λcont pd, to_expr ``(%%(pd.le pd.f₁ func_f) ∧ %%cont))
+        (pd.f₁.app_of_list pd.locals),
+      pds.mfoldl (λcont pd, to_expr ``(@Exists %%pd.type %%(cont.lambdas [pd.f₁]))) corec),
+    add_decl $ mk_definition pd.pred.const_name u_params (pd.type.pis $ params) $
+      pred_body.lambdas $ params ++ pd.locals,
 
-  /- prove `destruct` rule -/
-  destruct ← add_theorem_by (n ++ "destruct") us ((imp pred_gl func_pred_l).pis $ gs ++ ls) (do
-    gs ← intro_lst gs_names, ls ← intro_lst ls_names, h ← intro `h,
-    [([f, hf], [])] ← induction h [`f, `hf],
-    [([h₁, h₂], [])] ← induction hf [`h₁, `h₂],
-    apply $ mono.app_of_list $ gs ++ [f],
-    exact $ corec.app_of_list $ gs ++ [f, h₁],
-    exact $ h₁.app_of_list $ ls ++ [h₂]),
+    /- prove `corec_functional` rule -/
+    let corec_type := pds.foldl (λc pd, (pd.le pd.f₁ func_f).imp c) (pd.le pd.f₁ pd.pred_g),
+    add_theorem_by (pd.pred.const_name ++ "corec_functional") u_params (corec_type.pis $ params ++ f₁) (do
+      params ← intro_lst params_names,
+      fs ← intro_lst $ f₁.map local_pp_name,
+      hs ← intro_lst $ f₁.map (λf, mk_simple_name "hc"),
+      ls ← intro_lst $ pd.locals.map local_pp_name,
+      h ← intro `h,
+      whnf_target,
+      fs.mmap existsi,
+      hs.mmap (λf, constructor >> exact f),
+      exact h)),
+ 
+  let func_f := λpd : pred_predata, pd.func_g.app_of_list $ pds.map pred_predata.pred_g,
 
-  /- prove `construct` rule -/
-  let construct_type := (imp func_pred_l pred_gl).pis $ gs ++ ls,
-  construct ← add_theorem_by (n ++ "construct") us construct_type (do
-    gs ← intro_lst gs_names,
-    let pred := pred.app_of_list gs,
-    let func_pred := func.app_of_list $ gs ++ [pred],
-    apply $ corec.app_of_list $ gs ++ [func_pred],
-    apply $ mono.app_of_list $ gs ++ [pred, func_pred],
-    exact $ destruct.app_of_list gs),
+  /- prove `destruct` rules -/
+  pds.enum.mmap (λd:ℕ × pred_predata, do
+    let n := d.1,
+    let pd := d.2,
+    let destruct := (pd.le pd.pred_g (func_f pd)).pis $ params,
+    add_theorem_by (pd.pred.const_name ++ "destruct") u_params destruct (do
+      params ← intro_lst params_names,
+      ls ← intro_lst $ pd.locals.map local_pp_name,
+      h ← intro `h,
+      (fs, h) ← pds.mfoldl (λ(c:list expr × expr) (pd:pred_predata), do
+          [([f, hf], [])] ← induction c.2 [`f, `hf],
+          return (c.1 ++ [f], hf))
+        ([], h),
+      (hs, h) ← pds.mfoldl (λ(c:list expr × expr) (pd:pred_predata), do
+          [([h, h'], [])] ← induction c.2 [`h, `h'],
+          return (c.1 ++ [h], h'))
+        ([], h),
+      apply $ pd.mono.app_of_list $ params,
+      pds.mmap (λpd:pred_predata, focus1 $ do
+        apply $ pd.corec.app_of_list $ params,
+        focus $ hs.map exact),
+      some h' ← return $ hs.nth n,
+      apply h',
+      exact h)),
+
+  /- prove `construct` rules -/
+  pds.mmap (λpd:pred_predata,
+    add_theorem_by (pd.pred.const_name ++ "construct") u_params
+        ((pd.le (func_f pd) pd.pred_g).pis $ params) (do
+      params ← intro_lst params_names,
+      apply $ pd.corec.app_of_list $ params,
+      apply $ pd.mono.app_of_list $ params,
+      focus $ pds.map (λpd, apply pd.destruct))),
 
   /- prove constructors -/
-  irules.mmap (λ⟨nr, t⟩, add_theorem_by nr us t $ do
-    (name.mk_string sub p) ← return nr,
-    let func_rule : expr := (const ((p ++ "functional") ++ sub) us'),
-    gs ← intro_lst gs_names, bs ← intros,
-    apply $ construct.app_of_list $ gs,
-    exact $ func_rule.app_of_list $ gs ++ [pred.app_of_list gs] ++ bs),
+  pds.mmap (λpd:pred_predata, do
+    pd.intros.mmap (λ⟨nr, t⟩, do
+      let t : expr := expr.instantiate_locals (pds.map (λpd:pred_predata,
+        (pd.pd_name, (const pd.pd_name u_params').app_of_list params))) t,
+      add_theorem_by nr u_params (t.pis params) $ do
+      (name.mk_string sub p) ← return nr,
+      let func_rule : expr := (const ((p ++ "functional") ++ sub) u_params'),
+      params ← intro_lst params_names, bs ← intros,
+      apply $ pd.construct.app_of_list $ params,
+      exact $ func_rule.app_of_list $ params ++ [pd.pred.app_of_list params] ++ bs)),
 
   return ()
 
